PathDependent.lean
@@ -1,6 +1,7 @@
 -- This module serves as the root of the `PathDependent` library.
 -- Import modules here that should be built as part of the library.
 import «PathDependent».Basic
+import «PathDependent».FinFun.Basic
 import «PathDependent».LambdaP.Syntax
 import «PathDependent».LambdaP.Context
 import «PathDependent».LambdaP.Typing
