PathDependent/FinFun/Basic.lean
@@ -1,0 +1,52 @@
+import Mathlib.Init.Function
+
+def FinFun (n n' : Nat) : Type :=
+  Fin n -> Fin n'
+
+def FinFun.id : FinFun n n :=
+  fun i => i
+
+def FinFun.weaken : FinFun n (n+1) :=
+  Fin.succ
+
+theorem FinFun.weaken_inj {n : Nat} : Function.Injective (weaken (n := n)) := by
+  intro a b h
+  unfold weaken at h
+  simp [Fin.succ_inj] at h
+  trivial
+
+def FinFun.open (x : Fin n) : FinFun (n+1) n := by
+  intro i
+  cases i using Fin.cases
+  case zero => exact x
+  case succ j => exact j
+
+def FinFun.ext (f : FinFun n n') : FinFun (n+1) (n'+1) := by
+  intro i
+  cases i using Fin.cases
+  case zero => exact 0
+  case succ j => exact Fin.succ (f j)
+
+theorem FinFun.comp_weaken {f : FinFun n n'} :
+  weaken ∘ f = f.ext ∘ weaken := by
+  funext i
+  cases n
+  case zero => exact rfl
+  case succ =>
+    cases i using Fin.cases
+    case zero => exact rfl
+    case succ j => exact rfl
+
+theorem FinFun.ext_comp_ext {f : FinFun n n'} {g : FinFun n' n''} :
+  g.ext ∘ f.ext = FinFun.ext (g ∘ f) := by
+  funext i
+  cases i using Fin.cases
+  case zero => exact rfl
+  case succ j => exact rfl
+
+theorem FinFun.open_comp {f : FinFun n n'} {x : Fin n} :
+  f ∘ FinFun.open x = FinFun.open (f x) ∘ f.ext := by
+  funext i
+  cases i using Fin.cases
+  case zero => exact rfl
+  case succ j => exact rfl
